<?xml version="1.0"?>
<rdf:RDF xmlns="http://def.isotc211.org/geosciml/gsmle#"
     xml:base="http://def.isotc211.org/geosciml/gsmle"
     xmlns:rdf="http://www.w3.org/1999/02/22-rdf-syntax-ns#"
     xmlns:terms="http://purl.org/dc/terms/"
     xmlns:owl="http://www.w3.org/2002/07/owl#"
     xmlns:xml="http://www.w3.org/XML/1998/namespace"
     xmlns:xsd="http://www.w3.org/2001/XMLSchema#"
     xmlns:skos="http://www.w3.org/2004/02/skos/core#"
     xmlns:rdfs="http://www.w3.org/2000/01/rdf-schema#"
     xmlns:vann="http://purl.org/vocab/vann/"
     xmlns:dc="http://purl.org/dc/elements/1.1/">
    <owl:Ontology rdf:about="http://def.isotc211.org/geosciml/gsmle#">
        <owl:versionIRI rdf:resource="http://def.isotc211.org/geosciml/2018/gsmle#"/>
        <owl:imports rdf:resource="http://def.isotc211.org/geosciml/2018/gsmlb"/>
        <owl:imports rdf:resource="https://github.com/GeoscienceAustralia/geosciml.org/commit/24d302bf3f0fa315c1dddc2c734b84f52299cd02#diff-73b17e22072459ab7e06e9ab664a9d48"/>
    </owl:Ontology>
    


    <!-- 
    ///////////////////////////////////////////////////////////////////////////////////////
    //
    // Annotation properties
    //
    ///////////////////////////////////////////////////////////////////////////////////////
     -->

    


    <!-- http://www.w3.org/2004/02/skos/core#definition -->

    <owl:AnnotationProperty rdf:about="http://www.w3.org/2004/02/skos/core#definition"/>
    


    <!-- 
    ///////////////////////////////////////////////////////////////////////////////////////
    //
    // Classes
    //
    ///////////////////////////////////////////////////////////////////////////////////////
     -->

    


    <!-- http://def.isotc211.org/geosciml/gsmlb#EarthMaterial -->

    <owl:Class rdf:about="http://def.isotc211.org/geosciml/gsmlb#EarthMaterial"/>
    


    <!-- http://def.isotc211.org/geosciml/gsmlb#Foliation -->

    <owl:Class rdf:about="http://def.isotc211.org/geosciml/gsmlb#Foliation"/>
    


    <!-- http://def.isotc211.org/geosciml/gsmlb#GeologicEvent -->

    <owl:Class rdf:about="http://def.isotc211.org/geosciml/gsmlb#GeologicEvent"/>
    


    <!-- http://def.isotc211.org/geosciml/gsmlb#GeologicStructure -->

    <owl:Class rdf:about="http://def.isotc211.org/geosciml/gsmlb#GeologicStructure"/>
    


    <!-- http://def.isotc211.org/geosciml/gsmle##AbstractFeatureRelation -->

    <owl:Class rdf:about="http://def.isotc211.org/geosciml/gsmle##AbstractFeatureRelation">
        <rdfs:comment xml:lang="en">Association class placeholder to describe relations between geologic features.</rdfs:comment>
        <rdfs:label xml:lang="en">Abstract Feature Relation</rdfs:label>
    </owl:Class>
    


    <!-- http://def.isotc211.org/geosciml/gsmle##AlterationDescription -->

    <owl:Class rdf:about="http://def.isotc211.org/geosciml/gsmle##AlterationDescription">
        <rdfs:subClassOf rdf:resource="http://def.isotc211.org/geosciml/gsmle##EarthMaterialAbstractDescription"/>
        <rdfs:label xml:lang="en">Alteration Description</rdfs:label>
        <skos:definition xml:lang="en">AlterationDescription describes aspects of a geologic unit or earth material that are the result of bulk chemical, mineralogical or physical changes related to change in the physical or chemical environment. It includes weathering, supergene alteration, hydrothermal alteration and metasomatic effects not considered metamorphic. For example, a soil profile description would have to be constructed as a GeologicUnit (geologicUnitType = PedologicUnit) with unit parts representing the various horizons in the profile.  Thickness of a weathering profile can be delivered as unitThickness of a GeologicUnit of geologicUnitType equal to “AlterationUnit”</skos:definition>
    </owl:Class>
    


    <!-- http://def.isotc211.org/geosciml/gsmle##BeddingDescription -->

    <owl:Class rdf:about="http://def.isotc211.org/geosciml/gsmle##BeddingDescription">
        <rdfs:label xml:lang="en">Bedding Description</rdfs:label>
        <skos:definition xml:lang="en">BeddingDescription provides a detailed description of the bedding characteristics of a geologic unit.</skos:definition>
    </owl:Class>
    


    <!-- http://def.isotc211.org/geosciml/gsmle##ChemicalDescription -->

    <owl:Class rdf:about="http://def.isotc211.org/geosciml/gsmle##ChemicalDescription">
        <rdfs:subClassOf rdf:resource="http://def.isotc211.org/geosciml/gsmle##EarthMaterialAbstractDescription"/>
        <rdfs:label xml:lang="en">Chemical Description</rdfs:label>
        <skos:definition xml:lang="en">ChemicalComposition is a kind of EarthMaterialDescription that delivers the chemical composition of a geological unit or earth material, as a list of element or oxide concentrations.</skos:definition>
    </owl:Class>
    


    <!-- http://def.isotc211.org/geosciml/gsmle##CompoundMaterialDescription -->

    <owl:Class rdf:about="http://def.isotc211.org/geosciml/gsmle##CompoundMaterialDescription">
        <rdfs:subClassOf rdf:resource="http://def.isotc211.org/geosciml/gsmle##EarthMaterialAbstractDescription"/>
        <rdfs:label xml:lang="en">Compound Material Description</rdfs:label>
        <skos:definition xml:lang="en">The CompoundMaterialDescription class is a kind of EarthMaterialDescription that provides an extended description of a compound earth material (i.e., rocks and unconsolidated solid earth materials).</skos:definition>
    </owl:Class>
    


    <!-- http://def.isotc211.org/geosciml/gsmle##ConstituentPart -->

    <owl:Class rdf:about="http://def.isotc211.org/geosciml/gsmle##ConstituentPart">
        <rdfs:label xml:lang="en">Constituent Part</rdfs:label>
        <skos:definition xml:lang="en">The ConstituentPart class describes how Earth materials may be made up of other Earth materials, including the proportion of the constituent part in the whole (e.g., 20%, minor, dominant); and the role that the constituent plays in the whole (e.g., matrix, groundmass, framework, phenocryst, xenolith, vein).</skos:definition>
    </owl:Class>
    


    <!-- http://def.isotc211.org/geosciml/gsmle##ContactAbstractDescription -->

    <owl:Class rdf:about="http://def.isotc211.org/geosciml/gsmle##ContactAbstractDescription">
        <rdfs:label xml:lang="en">Contact Abstract Description</rdfs:label>
    </owl:Class>
    


    <!-- http://def.isotc211.org/geosciml/gsmle##ContactDescription -->

    <owl:Class rdf:about="http://def.isotc211.org/geosciml/gsmle##ContactDescription">
        <rdfs:subClassOf rdf:resource="http://def.isotc211.org/geosciml/gsmle##ContactAbstractDescription"/>
        <rdfs:label xml:lang="en">Contact Description</rdfs:label>
        <skos:definition xml:lang="en">The ContactDescription provides extended descriptive properties of a geologic contact.  If the contact type is ChronostratigraphicBoundary, it can be associated with a geochronologic (i.e., time zone) boundary that may correlate with it.</skos:definition>
    </owl:Class>
    


    <!-- http://def.isotc211.org/geosciml/gsmle##DisplacementEvent -->

    <owl:Class rdf:about="http://def.isotc211.org/geosciml/gsmle##DisplacementEvent">
        <rdfs:subClassOf rdf:resource="http://def.isotc211.org/geosciml/gsmlb#GeologicEvent"/>
        <rdfs:label xml:lang="en">Displacement Event</rdfs:label>
        <skos:definition xml:lang="en">A displacement event is a description of the age, environment and process of a shear displacement event.</skos:definition>
    </owl:Class>
    


    <!-- http://def.isotc211.org/geosciml/gsmle##DisplacementValue -->

    <owl:Class rdf:about="http://def.isotc211.org/geosciml/gsmle##DisplacementValue">
        <rdfs:subClassOf rdf:resource="http://def.isotc211.org/geosciml/gsmle##ShearDisplacementStructureAbstractDescription"/>
        <rdfs:label xml:lang="en">Displacement Value</rdfs:label>
        <skos:definition xml:lang="en">A displacement value expresses the displacement on a fault with respect to a planar approximation of its shape.</skos:definition>
    </owl:Class>
    


    <!-- http://def.isotc211.org/geosciml/gsmle##EarthMaterialAbstractDescription -->

    <owl:Class rdf:about="http://def.isotc211.org/geosciml/gsmle##EarthMaterialAbstractDescription">
        <rdfs:comment xml:lang="en">EarthMaterialDescription abstract class is materialised into a series of concrete classes to address various aspects of EarthMaterial descriptions:</rdfs:comment>
        <rdfs:label xml:lang="en">Earth Material Description</rdfs:label>
    </owl:Class>
    


    <!-- http://def.isotc211.org/geosciml/gsmle##FabricDescription -->

    <owl:Class rdf:about="http://def.isotc211.org/geosciml/gsmle##FabricDescription">
        <rdfs:subClassOf rdf:resource="http://def.isotc211.org/geosciml/gsmle##EarthMaterialAbstractDescription"/>
        <rdfs:label xml:lang="en">Fabric Description</rdfs:label>
        <skos:definition xml:lang="en">The FabricDescription data type describes all types of fabrics associated with a CompoundMaterial (i.e., tectonic, metamorphic, sedimentary, igneous fabrics or textures).  It denotes a pattern, defined by one or more CompoundMaterial constituents, that is present throughout a rock body when considered at some scale.  FabricDescription is defined based on the average configuration of many constituents.  Penetrative fabric denotes that these constituents are distributed throughout the rock volume at the scale of observation [15], and are repeated at distances that are small relative to the scale of the whole, such that they can be considered to pervade the whole uniformly</skos:definition>
    </owl:Class>
    


    <!-- http://def.isotc211.org/geosciml/gsmle##FoldAbstractDescription -->

    <owl:Class rdf:about="http://def.isotc211.org/geosciml/gsmle##FoldAbstractDescription">
        <rdfs:label xml:lang="en">Fold Abstract Description</rdfs:label>
        <skos:definition xml:lang="en">An abstract class providing a link between classes in GeoSciMLBasic and GeoSciMLExtended application schemas.</skos:definition>
    </owl:Class>
    


    <!-- http://def.isotc211.org/geosciml/gsmle##FoldDescription -->

    <owl:Class rdf:about="http://def.isotc211.org/geosciml/gsmle##FoldDescription">
        <rdfs:subClassOf rdf:resource="http://def.isotc211.org/geosciml/gsmle##FoldAbstractDescription"/>
        <rdfs:label xml:lang="en">Fold Description</rdfs:label>
        <skos:definition xml:lang="en">FoldDescription is an extended descriptive property of a fold structure.</skos:definition>
    </owl:Class>
    


    <!-- http://def.isotc211.org/geosciml/gsmle##FoldSystem -->

    <owl:Class rdf:about="http://def.isotc211.org/geosciml/gsmle##FoldSystem">
        <rdfs:subClassOf rdf:resource="http://def.isotc211.org/geosciml/gsmlb#GeologicStructure"/>
        <rdfs:label xml:lang="en">Fold System</rdfs:label>
        <skos:definition xml:lang="en">A FoldSystem is a collection of congruent folds (axis and axial surface are parallel) produced by the same tectonic event. It is sometimes referred to as a “fold train”.</skos:definition>
    </owl:Class>
    


    <!-- http://def.isotc211.org/geosciml/gsmle##FoliationAbstractDescription -->

    <owl:Class rdf:about="http://def.isotc211.org/geosciml/gsmle##FoliationAbstractDescription">
        <rdfs:label xml:lang="en">Foliation Abstract Description</rdfs:label>
        <skos:definition xml:lang="en">An abstract class providing a link between classes in GeoSciMLBasic and GeoSciMLExtended application schemas.</skos:definition>
    </owl:Class>
    


    <!-- http://def.isotc211.org/geosciml/gsmle##GeologicEventAbstractDescription -->

    <owl:Class rdf:about="http://def.isotc211.org/geosciml/gsmle##GeologicEventAbstractDescription">
        <rdfs:label xml:lang="en">Geologic Event Abstract Description</rdfs:label>
    </owl:Class>
    


    <!-- http://def.isotc211.org/geosciml/gsmle##GeologicEventDescription -->

    <owl:Class rdf:about="http://def.isotc211.org/geosciml/gsmle##GeologicEventDescription">
        <rdfs:subClassOf rdf:resource="http://def.isotc211.org/geosciml/gsmle##GeologicEventAbstractDescription"/>
        <rdfs:label xml:lang="en">Geologic Event Description</rdfs:label>
        <skos:definition xml:lang="en">GeologicEventDescription provides extended description of geologic events through links to GeochronologicEras in the GeologicTimescale model</skos:definition>
    </owl:Class>
    


    <!-- http://def.isotc211.org/geosciml/gsmle##GeologicFeatureRelation -->

    <owl:Class rdf:about="http://def.isotc211.org/geosciml/gsmle##GeologicFeatureRelation">
        <rdfs:subClassOf rdf:resource="http://def.isotc211.org/geosciml/gsmle##AbstractFeatureRelation"/>
        <rdfs:label xml:lang="en">Geologic Feature Relation</rdfs:label>
        <skos:definition xml:lang="en">The GeologicFeatureRelation class defines the general structure used to define relationships between any GeoSciML feature types.  Relationships are always binary and directional.  There is always a single source and a single target.  The relationship is always defined from the perspective of the Source and is generally an active verb.</skos:definition>
    </owl:Class>
    


    <!-- http://def.isotc211.org/geosciml/gsmle##GeologicUnitAbstractDescription -->

    <owl:Class rdf:about="http://def.isotc211.org/geosciml/gsmle##GeologicUnitAbstractDescription">
        <rdfs:label xml:lang="en">Geologic Unit Abstract Description</rdfs:label>
    </owl:Class>
    


    <!-- http://def.isotc211.org/geosciml/gsmle##GeologicUnitDescription -->

    <owl:Class rdf:about="http://def.isotc211.org/geosciml/gsmle##GeologicUnitDescription">
        <rdfs:subClassOf rdf:resource="http://def.isotc211.org/geosciml/gsmle##GeologicUnitAbstractDescription"/>
        <rdfs:label xml:lang="en">Geologic Unit Description</rdfs:label>
        <skos:definition xml:lang="en">GeologicUnitDescription provides for extended description of the characteristics of a geologic unit</skos:definition>
    </owl:Class>
    


    <!-- http://def.isotc211.org/geosciml/gsmle##InorganicFluid -->

    <owl:Class rdf:about="http://def.isotc211.org/geosciml/gsmle##InorganicFluid">
        <rdfs:subClassOf rdf:resource="http://def.isotc211.org/geosciml/gsmlb#EarthMaterial"/>
        <rdfs:label xml:lang="en">Inorganic Fluid</rdfs:label>
        <skos:definition xml:lang="en">An inorganic fluid is a non-crystalline EarthMaterial (solid, liquid, or gas) that tends to flow or conform to the shape of its container (examples: water, brine, glass)..  By convention liquid mercury is considered a mineral.   This class is an empty placeholder for extension at a later date, or by other domain models.</skos:definition>
    </owl:Class>
    


    <!-- http://def.isotc211.org/geosciml/gsmle##Layering -->

    <owl:Class rdf:about="http://def.isotc211.org/geosciml/gsmle##Layering">
        <rdfs:subClassOf rdf:resource="http://def.isotc211.org/geosciml/gsmlb#Foliation"/>
        <rdfs:label xml:lang="en">Layering</rdfs:label>
        <skos:definition xml:lang="en">A planar foliation is defined by a tabular succession of layers &gt; 5 mm thick. This definition is based on the proposed definition of gneiss by the NADM Science Language Technical Team.  The GeologicStructure characteristic of gneiss is layering.</skos:definition>
    </owl:Class>
    


    <!-- http://def.isotc211.org/geosciml/gsmle##MaterialRelation -->

    <owl:Class rdf:about="http://def.isotc211.org/geosciml/gsmle##MaterialRelation">
        <rdfs:comment xml:lang="en">The MaterialRelation class describes the relationships between constituent parts in an EarthMaterial (e.g. A mineral overgrowth on a phenocryst within a granite).</rdfs:comment>
        <rdfs:label xml:lang="en">Material Relation</rdfs:label>
    </owl:Class>
    


    <!-- http://def.isotc211.org/geosciml/gsmle##MetamorphicDescription -->

    <owl:Class rdf:about="http://def.isotc211.org/geosciml/gsmle##MetamorphicDescription">
        <rdfs:subClassOf rdf:resource="http://def.isotc211.org/geosciml/gsmle##EarthMaterialAbstractDescription"/>
        <rdfs:label xml:lang="en">Metamorphic Description</rdfs:label>
        <skos:definition xml:lang="en">The data type MetamorphicDescription describes the character of metamorphism applied to a CompoundMaterial or GeologicUnit using one or more properties including estimated intensity (grade; e.g. high grade, low grade), characteristic metamorphic mineral assemblages (facies; e.g., greenschist, amphibolite), peak P-T estimates, and protolith material if known.  A MetamorphicDescription provides a link to the GeologicEvent associated to the metamorphic event.</skos:definition>
    </owl:Class>
    


    <!-- http://def.isotc211.org/geosciml/gsmle##Mineral -->

    <owl:Class rdf:about="http://def.isotc211.org/geosciml/gsmle##Mineral">
        <rdfs:subClassOf rdf:resource="http://def.isotc211.org/geosciml/gsmlb#EarthMaterial"/>
        <rdfs:label xml:lang="en">Mineral</rdfs:label>
        <skos:definition xml:lang="en">A naturally occurring inorganic element or compound having a periodically repeating arrangement of atoms and a characteristic chemical composition or range of compositions, resulting in distinctive physical properties.  Includes mercury as a general exception to the requirement of crystallinity.  Also includes crypto-crystalline materials such as chalcedony and amorphous silica.</skos:definition>
    </owl:Class>
    


    <!-- http://def.isotc211.org/geosciml/gsmle##NetSlipValue -->

    <owl:Class rdf:about="http://def.isotc211.org/geosciml/gsmle##NetSlipValue">
        <rdfs:subClassOf rdf:resource="http://def.isotc211.org/geosciml/gsmle##DisplacementValue"/>
        <rdfs:label xml:lang="en">Net Slip Value</rdfs:label>
        <skos:definition xml:lang="en">NetSlipValue is a kind of DisplacementValue that describes the total amount of slip displacement along a structure.</skos:definition>
    </owl:Class>
    


    <!-- http://def.isotc211.org/geosciml/gsmle##OrganicMaterial -->

    <owl:Class rdf:about="http://def.isotc211.org/geosciml/gsmle##OrganicMaterial">
        <rdfs:subClassOf rdf:resource="http://def.isotc211.org/geosciml/gsmlb#EarthMaterial"/>
        <rdfs:label xml:lang="en">Organic Material</rdfs:label>
        <skos:definition xml:lang="en">OrganicMaterial is an EarthMaterial that belongs to the class of chemical compounds having a reduced carbon basis (as distinct from carbonates), and derived from living organisms. It includes high-carbon EarthMaterials such as bitumen, peat, and coal.  This class is an empty placeholder for extension at a later date, or by other domain models.</skos:definition>
    </owl:Class>
    


    <!-- http://def.isotc211.org/geosciml/gsmle##Organism -->

    <owl:Class rdf:about="http://def.isotc211.org/geosciml/gsmle##Organism">
        <rdfs:label xml:lang="en">Organism</rdfs:label>
        <skos:definition xml:lang="en">Organism is a broad class to represent any living or once living things. This is the connection to taxonomy/biology for fossils.  This class is an empty placeholder for extension at a later date, or by other domain models.</skos:definition>
    </owl:Class>
    


    <!-- http://def.isotc211.org/geosciml/gsmle##ParticleGeometryDescription -->

    <owl:Class rdf:about="http://def.isotc211.org/geosciml/gsmle##ParticleGeometryDescription">
        <rdfs:label xml:lang="en">Particle Geometry Description</rdfs:label>
        <skos:definition xml:lang="en">ParticleGeometryDescription describes particles in a CompoundMaterial independent of their relationship to each other or their orientation. It is distinguished from Fabric in that the ParticleGeometryDescription remains constant if the material is disaggregated into its constituent particles, whereas Fabric is lost if the material is disaggregated.  Properties include the particle size (grainsize), particle sorting (size distribution, e.g., well sorted, poorly sorted, bimodal sorting), particle shape (surface rounding or crystal face development, e.g., well rounded, euhedral, anhedral), and particle aspect ratio (e.g., elongated, platy, bladed, compact, acicular).</skos:definition>
    </owl:Class>
    


    <!-- http://def.isotc211.org/geosciml/gsmle##PhysicalDescription -->

    <owl:Class rdf:about="http://def.isotc211.org/geosciml/gsmle##PhysicalDescription">
        <rdfs:subClassOf rdf:resource="http://def.isotc211.org/geosciml/gsmle##EarthMaterialAbstractDescription"/>
        <rdfs:label xml:lang="en">Physical Description</rdfs:label>
        <skos:definition xml:lang="en">PhysicalDescription is a class that describes the numeric physical properties of a geologic unit, earth material , or geologic structure, (e.g., density, porosity, magnetic susceptibility, remanent magnetism).  These properties are modelled here as scalar numeric values.</skos:definition>
    </owl:Class>
    


    <!-- http://def.isotc211.org/geosciml/gsmle##RockMaterialDescription -->

    <owl:Class rdf:about="http://def.isotc211.org/geosciml/gsmle##RockMaterialDescription">
        <rdfs:subClassOf rdf:resource="http://def.isotc211.org/geosciml/gsmle##EarthMaterialAbstractDescription"/>
        <rdfs:label xml:lang="en">Rock Material Description</rdfs:label>
        <skos:definition xml:lang="en">RockMaterialDescription provides extended description of RockMaterial.</skos:definition>
    </owl:Class>
    


    <!-- http://def.isotc211.org/geosciml/gsmle##SeparationValue -->

    <owl:Class rdf:about="http://def.isotc211.org/geosciml/gsmle##SeparationValue">
        <rdfs:subClassOf rdf:resource="http://def.isotc211.org/geosciml/gsmle##DisplacementValue"/>
        <rdfs:label xml:lang="en">Separation Value</rdfs:label>
        <skos:definition xml:lang="en">SeparationValue is a kind of DisplacementValue that describes the amount of separation displacement across a structure.</skos:definition>
    </owl:Class>
    


    <!-- http://def.isotc211.org/geosciml/gsmle##ShearDisplacementStructureAbstractDescription -->

    <owl:Class rdf:about="http://def.isotc211.org/geosciml/gsmle##ShearDisplacementStructureAbstractDescription">
        <rdfs:label xml:lang="en">Shear Displacement Structure Abstract Description</rdfs:label>
        <skos:definition xml:lang="en">An abstract class providing a link between classes in GeoSciMLBasic and GeoSciMLExtended application schemas.</skos:definition>
    </owl:Class>
    


    <!-- http://def.isotc211.org/geosciml/gsmle##SlipComponents -->

    <owl:Class rdf:about="http://def.isotc211.org/geosciml/gsmle##SlipComponents">
        <rdfs:subClassOf rdf:resource="http://def.isotc211.org/geosciml/gsmle##DisplacementValue"/>
        <rdfs:label xml:lang="en">Slip Components</rdfs:label>
        <skos:definition xml:lang="en">SlipComponents is a kind of DisplacementValue that is a representation of slip as a vector resolved into components within a reference frame in which horizontal axes are parallel and perpendicular to the strike of the fault.  At least one of heave, horizontalSlip, or throw must not be null.</skos:definition>
    </owl:Class>
</rdf:RDF>



<!-- Generated by the OWL API (version 4.2.8.20170104-2310) https://github.com/owlcs/owlapi -->

