@prefix owl: <http://www.w3.org/2002/07/owl#> .
@prefix rdfs: <http://www.w3.org/2000/01/rdf-schema#> .
@prefix skos: <http://www.w3.org/2004/02/skos/core#> .
@prefix gwmlc: <http://def.isotc211.org/gwml/gwmlc#>.

gwmlc:
  a owl:Ontology ;
  owl:versionIRI <http://def.isotc211.org/gwml/2018/gwmlc#> ;
  owl:imports <http://def.isotc211.org/geosciml/2018/gsmlc#> .
  
gwmlc:GW_Constituent 
	a owl:Class;
	rdfs:subClassOf <http://def.isotc211.org/iso19109/2015/GeneralFeatureModel#AnyFeature>;
	rdfs:label "Constituent"@en;
	skos:definition "General (abstract) entity denoting a material, chemical or biological constituent of a fluid body."@en.

gwmlc:GW_BiologicConstituent
	a owl:Class;
	rdfs:subClassOf gwmlc:GW_Constitent;
	rdfs:label "Biologic Constiuent "@en;
	skos:definition "Characterisation of the biological composition of the fluid body, both natural and man-made."@en.
	
gwmlc:GW_ChemicalConstituent
	a owl:Class;
	rdfs:subClassOf gwmlc:GW_Constituent;
	rdfs:label "Chemical Constituent"@en;
	skos:definition "Characterisation of the chemical composition of the fluid body, both natural and man-made."@en.
	
gwmlc:GW_MaterialConstituent
	a owl:Class;
	rdfs:subClassOf gwmlc:GW_Constituent;
	rdfs:label "Material Constituent"@en;
	skos:definition "Suspende or colloidal material in a fluid body, e.g sediment. "@en.
	
